src/vminus/Atom.v
@@ -1,0 +1,79 @@
+(* TODO:
+   -  Use MetatheoryAtom instead of this one.
+   -  license
+*)
+
+
+
+
+(** This file defines a type of atoms with: 
+      - a _decidable equality_ 
+      - a way of generating _fresh_ atoms
+*)
+
+
+
+Require Import Arith List Equalities PeanoNat.
+
+(** ** ATOM *)
+
+Module Type ATOM <: UsualDecidableType.
+
+  Parameter t : Set.
+  Parameter eq_dec : forall (x y:t), {x = y} + {x <> y}.
+  Parameter fresh : list t -> t.
+  Parameter fresh_not_in : forall l, ~ In (fresh l) l.
+
+  Include HasUsualEq <+ UsualIsEq.
+
+End ATOM.
+
+(** ** Atom *)
+(** Implements the [ATOM] signature. *)
+
+Module Atom : ATOM.
+
+  Definition t := nat.
+  Definition eq_dec := eq_nat_dec.
+  
+  Fixpoint max_elt (al:list t) : t :=
+    match al with
+      | nil => 0
+      | n'::al' => max n' (max_elt al')
+    end.
+
+  Definition fresh (al:list t) : t :=
+    S (max_elt al).
+
+  Lemma max_elt_spec : forall al b,
+    In b al -> b <= max_elt al.
+(* FOLD *)
+  Proof.
+    intros. induction al. inversion H.
+      inversion H; subst; simpl. apply Nat.le_max_l.
+      eapply le_trans; auto with arith. apply Nat.le_max_r.
+  Qed.
+(* /FOLD *)
+    
+  Lemma fresh_not_in : forall l, 
+    ~ In (fresh l) l.
+(* FOLD *)
+  Proof.
+    unfold fresh, not. intros l Hin.
+    specialize (max_elt_spec _ _ Hin). intro Ha.
+    contradict Ha; apply le_Sn_n.
+  Qed.
+(* /FOLD *)
+
+  Include HasUsualEq <+ UsualIsEq.
+
+End Atom.
+
+(* Automatically unfold Atom.eq *)
+Global Arguments Atom.eq /.
+
+
+
+
+
+
