src/vminus/Env.v
@@ -1,0 +1,78 @@
+(* -------------------------------------------------------------------------- *
+ *                     Vellvm - the Verified LLVM project                     *
+ *                                                                            *
+ *     Copyright (c) 2017 Steve Zdancewic <stevez@cis.upenn.edu>              *
+ *                                                                            *
+ *   This file is distributed under the terms of the GNU General Public       *
+ *   License as published by the Free Software Foundation, either version     *
+ *   3 of the License, or (at your option) any later version.                 *
+ ---------------------------------------------------------------------------- *)
+
+
+(** * Environments *)
+
+Require Import Equalities List.
+Set Implicit Arguments.
+
+(** An _environment_ maps values of type [K.t] to values of type 
+    V. This module implements updateable environments using Coq 
+    functions and proves some simple facts about equality. *)
+
+Module Make_Env (K:UsualDecidableType).
+Section WithV.
+  Variable V : Type.
+
+  Definition t := K.t -> V.
+
+  Definition empty (init:V) : t := fun _ => init.
+
+  Definition update (st:t) (k:K.t) (v:V) : t :=
+    fun k' => if K.eq_dec k k' then v else st k'.
+
+  (* Properties *)
+  Theorem update_eq : forall v k1 k2 st,
+    K.eq k1 k2 -> (update st k1 v) k2 = v.
+(* FOLD *)
+  Proof.
+    intros. unfold update. 
+    destruct (K.eq_dec k1 k2); intuition.
+  Qed.
+(* /FOLD *)
+
+  Theorem update_neq : forall k1 k2 v st,
+    ~ K.eq k1 k2 -> (update st k1 v) k2 = st k2.
+(* FOLD *)
+  Proof.
+    intros. unfold update.
+    destruct (K.eq_dec k1 k2); intuition.
+  Qed.
+(* /FOLD *)
+
+  Theorem update_shadow : forall v1 v2 k1 k2 st,
+    K.eq k1 k2 -> 
+    (update (update st k1 v1) k1 v2) k2 = (update st k1 v2) k2.
+(* FOLD *)
+  Proof.
+    intros. unfold update.
+    destruct (K.eq_dec k1 k2); reflexivity.
+  Qed.
+(* /FOLD *)
+
+  Theorem update_same : forall v1 k1 k2 (st : t),
+    st k2 = v1 -> (update st k1 v1) k2 = st k2.
+(* FOLD *)
+  Proof.
+    intros. unfold update. 
+    destruct (K.eq_dec k1 k2); subst; reflexivity.
+  Qed.
+(* /FOLD *)
+
+  Fixpoint mupdate (st:t) (ks:list K.t) (vs:list V) : t :=
+    match ks, vs with
+      | k :: ks', v :: vs' => mupdate (update st k v) ks' vs'
+      | _, _ => st
+    end.
+
+End WithV.
+End Make_Env.
+
