src/vminus/Imp.v
@@ -1,0 +1,159 @@
+(* TODO: License / Which Version of Imp? *)
+
+
+(** * Imp: Simple Imperative Programs *)
+
+(** FULL: This file presents a variant of the Imp programming language 
+    adapted from the Software Foundations book.  It is the source
+    language that will be compiled to the Vminus intermediate language
+    in this development.
+*)
+
+Require Import Equalities Arith.
+Require Import Vminus.Atom Env.
+
+(** *** Identifiers *)
+
+(** FULL: To simplify the compilation process, this variant of Imp uses 
+    [Atom.t] values as variable identifiers.  [Atom.t] is also used by
+    the [Vminus] language, so making them the same avoids the need to
+    use some kind of mapping from source to target identifiers.
+
+    This is a slight deviation from the earlier presentation that took
+    [id] to be constructed via [Id : nat -> id].  
+
+    The reason to use [Atom.t] is that this type supports the
+    generation of "fresh" identifiers, a feature needed in
+    implementing a compiler.  
+*)
+(** TERSE: One difference in this version of Imp: identifiers are given by [Atom.t].
+*)
+
+Definition id := Atom.t.
+
+(** TERSE:     This is a slight deviation from the earlier presentation that took
+    [id] to be constructed via [Id : nat -> id].  
+*)
+
+(** *** Arithmetic expressions *)
+(** Arithmetic expressions are just the same as in Imp. *)
+
+Inductive aexp : Type := 
+  | ANum   : nat -> aexp
+  | AId    : id -> aexp
+  | APlus  : aexp -> aexp -> aexp
+  | AMinus : aexp -> aexp -> aexp
+  | AMult  : aexp -> aexp -> aexp.
+
+(** *** Boolean expressions *)
+(** Boolean expressions are also just the same as in Imp.  Since (as
+    we'll see) Vminus doesn't support boolean values natively, we'll
+    have to compile these to natural numbers. *)
+
+Inductive bexp : Type := 
+  | BTrue  : bexp
+  | BFalse : bexp
+  | BEq    : aexp -> aexp -> bexp
+  | BLe    : aexp -> aexp -> bexp
+  | BNot   : bexp -> bexp
+  | BAnd   : bexp -> bexp -> bexp.
+
+(** *** Commands *)
+(** The commands are just the same as in Imp. *)
+
+Inductive com : Type :=
+  | CSkip : com
+  | CAss : id -> aexp -> com
+  | CSeq : com -> com -> com
+  | CIf : bexp -> com -> com -> com
+  | CWhile : bexp -> com -> com.
+
+
+(** *** Notation *)
+Notation "'SKIP'" := 
+  CSkip : imp_scope.
+Notation "X '::=' a" := 
+  (CAss X a) (at level 60) : imp_scope.
+Notation "c1 ;; c2" := 
+  (CSeq c1 c2) (at level 80, right associativity) : imp_scope.
+Notation "'WHILE' b 'DO' c 'END'" := 
+  (CWhile b c) (at level 80, right associativity) : imp_scope.
+Notation "'IFB' e1 'THEN' e2 'ELSE' e3 'FI'" := 
+  (CIf e1 e2 e3) (at level 80, right associativity) : imp_scope.
+
+(* FIX: Add an example program *)
+(** *** An Example:
+<<
+X ::= 5;;
+Y ::= 1;;
+WHILE (BNot (Beq (AId X) (ANum 0))) DO
+  Y ::= AMult (AId Y) (AId X);;         (* Y = Y * X *)
+  X ::= AMinus (AId X) (ANum 1)         (* X = X - 1 *)
+END
+>>
+*)
+
+(** ** Operational Semantics *)
+
+(** The _state_ of an Imp program maps Atoms to natural numbers. *)
+
+Module State := Make_Env Atom.
+
+Local Open Scope imp_scope.
+Definition state := State.t nat.
+Definition update := @State.update nat.
+
+
+(** *** Arithmetic evaluation *)
+(** Arithmetic and boolean expressions are evaluated in a given 
+    state. *)
+
+Fixpoint aeval (e : aexp) (st : state) : nat :=
+  match e with
+  | ANum n        => n
+  | AId X         => st X
+  | APlus a1 a2   => (aeval a1 st) + (aeval a2 st)
+  | AMinus a1 a2  => (aeval a1 st) - (aeval a2 st)
+  | AMult a1 a2   => (aeval a1 st) * (aeval a2 st)
+  end.
+
+
+(** *** Boolean evaluation *)
+Fixpoint beval (e : bexp) (st : state) : bool :=
+  match e with 
+  | BTrue       => true
+  | BFalse      => false
+  | BEq a1 a2   => beq_nat (aeval a1 st) (aeval a2 st)
+  | BLe a1 a2   => leb (aeval a1 st) (aeval a2 st)
+  | BNot b1     => negb (beval b1 st)
+  | BAnd b1 b2  => andb (beval b1 st) (beval b2 st)
+  end.
+
+
+(** *** Small step evaluation relation *)
+
+Inductive step : (com * state) -> (com * state) -> Prop :=
+| S_Ass : forall st i a n,
+    aeval a st = n ->
+    step (i ::= a, st) (SKIP, update st i n)
+
+| S_Seq : forall st st' c1 c1' c2,
+    step (c1, st) (c1', st') ->
+    step (c1 ;; c2, st) (c1' ;; c2, st')
+
+| S_SeqSkip : forall st c2,
+    step (SKIP ;; c2, st) (c2, st)
+
+| S_IfTrue : forall st c1 c2 e,
+    beval e st = true -> 
+    step (IFB e THEN c1 ELSE c2 FI, st) (c1, st)
+
+| S_IfFalse : forall st c1 c2 e,
+    beval e st = false ->
+    step (IFB e THEN c1 ELSE c2 FI, st) (c2, st)
+
+| S_While : forall st c e,
+    step (WHILE e DO c END, st) 
+         (IFB e THEN (c ;; WHILE e DO c END) ELSE SKIP FI, st).
+
+
