src/vminus/Iteration.v
@@ -1,0 +1,95 @@
+(* *********************************************************************)
+(*                                                                     *)
+(*              The Compcert verified compiler                         *)
+(*                                                                     *)
+(*          Xavier Leroy, INRIA Paris-Rocquencourt                     *)
+(*                                                                     *)
+(*  Copyright Institut National de Recherche en Informatique et en     *)
+(*  Automatique.  All rights reserved.  This file is distributed       *)
+(*  under the terms of the GNU General Public License as published by  *)
+(*  the Free Software Foundation, either version 2 of the License, or  *)
+(*  (at your option) any later version.  This file is also distributed *)
+(*  under the terms of the INRIA Non-Commercial License Agreement.     *)
+(*                                                                     *)
+(* *********************************************************************)
+(* -------------------------------------------------------------------------- *
+ *                     Vellvm - the Verified LLVM project                     *
+ *                                                                            *
+ *     Copyright (c) 2017 Steve Zdancewic <stevez@cis.upenn.edu>              *
+ *                                                                            *
+ *   This file is distributed under the terms of the GNU General Public       *
+ *   License as published by the Free Software Foundation, either version     *
+ *   3 of the License, or (at your option) any later version.                 *
+ ---------------------------------------------------------------------------- *)
+
+
+(** Bounded iterators *)
+
+(* we can get away with using unary nats in our toy compiler
+   Q: why does compcert use positive vs. binary nats? 
+      how are they extracted -- extra cons for each number?
+   binary nats are better supported in the stdlib*)
+
+Require Import NArith FunctionalExtensionality.
+
+Set Implicit Arguments.
+
+Module Iter.
+
+Section ITERATION.
+
+Variables A B: Type.
+Variable step: A -> B + A.
+
+Definition num_iterations := 1000000000000%N.
+
+Open Scope N_scope.
+
+Definition iter_step (x: N)
+                     (next: forall y, y < x -> A -> option B)
+                     (s: A) : option B :=
+  match N.eq_dec x N.zero with
+  | left EQ => None
+  | right NOTEQ =>
+      match step s with
+      | inl res => Some res
+      | inr s'  => next (N.pred x) (N.lt_pred_l x NOTEQ) s'
+      end
+  end.
+
+
+Definition iter: N -> A -> option B := Fix N.lt_wf_0 _ iter_step.
+Definition iterate := iter num_iterations.
+
+Variable P: A -> Prop.
+Variable Q: B -> Prop.
+
+Hypothesis step_prop:
+  forall a : A, P a ->
+  match step a with inl b => Q b | inr a' => P a' end.
+
+Lemma iter_prop:
+  forall n b a, P a -> iter n a = Some b -> Q b.
+Proof.
+  intros n b. pattern n. apply (well_founded_ind N.lt_wf_0).
+  intros until 2. rewrite (Fix_eq N.lt_wf_0 _ iter_step). 
+  unfold iter_step at 1. destruct (N.eq_dec _ _). 
+  discriminate 1. specialize (step_prop H0).
+  destruct (step a).
+    inversion 1; subst b0; exact step_prop.
+    apply H; auto. apply N.lt_pred_l; auto.
+  intros. f_equal. 
+  apply functional_extensionality_dep. intro. 
+  apply functional_extensionality_dep. auto.
+Qed.
+
+Lemma iterate_prop:
+  forall a b, iterate a = Some b -> P a -> Q b.
+Proof.
+  intros. apply iter_prop with num_iterations a; assumption.
+Qed.
+
+End ITERATION.
+
+End Iter.
+
