src/vminus/Kildall.v
@@ -1,0 +1,316 @@
+(* *********************************************************************)
+(*                                                                     *)
+(*              The Compcert verified compiler                         *)
+(*                                                                     *)
+(*          Xavier Leroy, INRIA Paris-Rocquencourt                     *)
+(*                                                                     *)
+(*  Copyright Institut National de Recherche en Informatique et en     *)
+(*  Automatique.  All rights reserved.  This file is distributed       *)
+(*  under the terms of the GNU General Public License as published by  *)
+(*  the Free Software Foundation, either version 2 of the License, or  *)
+(*  (at your option) any later version.  This file is also distributed *)
+(*  under the terms of the INRIA Non-Commercial License Agreement.     *)
+(*                                                                     *)
+(* *********************************************************************)
+(* -------------------------------------------------------------------------- *
+ *                     Vellvm - the Verified LLVM project                     *
+ *                                                                            *
+ *     Copyright (c) 2017 Steve Zdancewic <stevez@cis.upenn.edu>              *
+ *                                                                            *
+ *   This file is distributed under the terms of the GNU General Public       *
+ *   License as published by the Free Software Foundation, either version     *
+ *   3 of the License, or (at your option) any later version.                 *
+ ---------------------------------------------------------------------------- *)
+
+(* Acknowledgements --------------------------------------------------------- *)
+(* 
+  This file is heavily based on:
+      - lib/Lattice.v 
+      - backend/Kildall.v 
+  from the CompCert development,  modified to remove dependencies and 
+  optimizations.
+*)
+
+Require Import Equalities Orders.
+Require Import FSets FMaps.
+
+Require Import Iteration Util.
+
+Module Type FORWARD_SOLVER.
+
+  Declare Module L : LATTICE.             (* domain of approximations *)
+  Declare Module N : UsualDecidableType.  (* program points *)
+
+  Declare Module NM : FMapInterface.WSfun N.
+  Module FMP := FMapProps N NM.
+
+  Include EqLeNotation L.
+  Notation "a !! b" := (FMP.find_default a b L.bot) 
+                         (at level 1, format "a !! b").
+  Notation nlmap := (NM.t L.t).
+
+  Parameter fixpoint: forall 
+    (succs: N.t -> list N.t)
+    (trans: N.t -> L.t -> L.t)
+    (inits: nlmap),
+    option nlmap.
+
+  Axiom fixpoint_solution : forall succs trans inits res n s,
+    fixpoint succs trans inits = Some res ->
+    NM.In n inits ->
+    In s (succs n) ->
+    trans n res!!n <= res!!s.
+
+  Axiom fixpoint_entry : forall succs trans inits res n,
+    fixpoint succs trans inits = Some res ->
+    inits!!n <= res!!n.
+
+  Axiom fixpoint_invariant : forall succs trans inits
+    (P: N.t -> L.t -> Prop)
+    (Pinits: forall n, P n inits!!n)
+    (Ptrans: forall n ln s ls, 
+      In s (succs n) -> 
+      P n ln -> P s ls -> P s (L.join ls (trans n ln))),
+    forall res n, fixpoint succs trans inits = Some res -> P n res!!n.
+
+End FORWARD_SOLVER.
+
+Module ForwardSolver (PC:UsualDecidableType) (LAT:LATTICE):
+                     FORWARD_SOLVER with Module L := LAT
+                                    with Module N := PC.
+
+  Module L := LAT.
+  Module N := PC.
+  
+  Include EqLeNotation L.
+
+  (* TODO: can define a total order for PCs to use more efficient sets/maps *)
+  Module NM := FMapWeakList.Make N.
+  Module Import FMP := FMapProps N NM.
+  Module NMFacts := FMapFacts.WFacts NM.
+
+  Include EqLeNotation L.
+  Notation "a !! b" := (find_default a b L.bot) (at level 1, format "a !! b").
+  Notation nlmap := (NM.t L.t).
+
+  Record state := mkst { lmap: NM.t L.t; wlist: list N.t }.
+
+  Section KILDALL.
+
+  Variable succs : N.t -> list N.t.
+  Variable trans : N.t -> L.t -> L.t.
+  Variable inits : nlmap.
+
+  Definition prop_succ (out:L.t) (s:state) (n:N.t) : state :=
+    let oldl := s.(lmap)!!n in
+    let newl := L.join oldl out in
+    if L.eq_dec oldl newl 
+    then s else mkst (NM.add n newl s.(lmap)) (n::s.(wlist)).
+
+  Definition step (s:state) : NM.t L.t + state :=
+    match s.(wlist) with
+      | nil => inl s.(lmap)
+      | n::rem => 
+        inr (fold_left (prop_succ (trans n s.(lmap)!!n))
+                       (succs n) (mkst s.(lmap) rem))
+    end.
+
+  Definition make_init_state : state :=
+    mkst inits (map (@fst _ _) (NM.elements inits)).
+  
+  Definition fixpoint := Iter.iterate step make_init_state.
+
+
+  (* correctness *)
+
+  Definition n_invar (s:state) (n:N.t) : Prop :=
+    In n s.(wlist) \/ forall m, In m (succs n) -> 
+      trans n s.(lmap)!!n <= s.(lmap)!!m.
+
+  Definition state_invar (s:state) : Prop :=
+    forall n, NM.In n inits -> n_invar s n.
+
+  Lemma prop_n_invar_pres : forall o s n n',
+    n_invar s n -> n_invar (prop_succ o s n') n.
+  Proof.
+    unfold n_invar. intros.
+    set (s' := prop_succ o s n'); unfold prop_succ in s'.
+    destruct (L.eq_dec _ _). apply H.
+    destruct H. simpl; intuition.
+      destruct (N.eq_dec n n').
+        simpl; intuition. right. intros. 
+        destruct (N.eq_dec n' m); subst s'; simpl.
+          rewrite find_default_neq, find_default_eq; auto. 
+            transitivity (lmap s)!!m. apply H; auto. 
+            subst n'; apply L.le_join_l.
+          rewrite find_default_neq, find_default_neq; auto.
+  Qed.
+
+  Lemma prop_n_out : forall o ns s s' n,
+    s' = fold_left (prop_succ o) ns s ->
+    ~ In n (wlist s') ->
+    trans n (lmap s')!!n == trans n (lmap s)!!n.
+  Proof.
+    intros o ns s s' n Heqs'. pattern s'.
+    eapply fold_left_1; eauto.
+    intros. set (r := prop_succ o a b) in *.
+    unfold prop_succ in r. destruct (L.eq_dec _ _). apply H0; auto.
+    destruct (N.eq_dec b n). contradict H1; simpl; auto.
+      subst r. simpl in *. rewrite find_default_neq; auto.
+   intro. reflexivity.
+  Qed.
+
+  Lemma step_state_invar : forall s s',
+    state_invar s -> inr s' = step s -> state_invar s'.
+  Proof.
+    unfold step, state_invar; intros s s' Hinv Hstep. 
+    destruct (wlist s) eqn:Hwls. discriminate Hstep.
+    injection Hstep; clear Hstep. intros Heqs' n.
+
+    destruct (N.eq_dec t n).
+
+    (* n_invar is restablished for n *)
+    subst t. unfold n_invar. 
+    destruct(in_dec N.eq_dec n (wlist s')) as [|Hwl]; [auto | right].
+    intros m Hin. rewrite prop_n_out; eauto; simpl.
+    generalize Hwl; clear Hwl. pattern s', m.
+
+    eapply fold_left_2; eauto.
+      intros a b b'.
+      set (r := prop_succ _ a b').
+      intros. unfold prop_succ in r. destruct (L.eq_dec _ _). apply H0; auto.
+      unfold r. simpl. destruct (N.eq_dec b' b). 
+        rewrite find_default_eq; auto. apply L.le_join_r.
+        rewrite find_default_neq; auto. apply H0. contradict Hwl; simpl; auto.
+
+      intros a b.
+      set (r := prop_succ _ a b).
+      intros. unfold prop_succ in r. destruct (L.eq_dec _ _) as [Heq|].
+      subst r. rewrite Heq. apply L.le_join_r.
+      simpl. rewrite find_default_eq; auto. apply L.le_join_r.
+
+    (* n_invar is preserved for all successors ~= n *)
+    intros Hin. pattern s'. eapply fold_left_1; eauto.
+    intros. apply prop_n_invar_pres. assumption.
+    unfold state_invar, n_invar in Hinv |- *.
+    simpl. specialize (Hinv n). rewrite Hwls in Hinv. destruct Hinv.
+    assumption. left. destruct H; intuition. right. apply H.
+  Qed. 
+
+  Lemma fixpoint_solution: forall res n s,
+    fixpoint = Some res ->
+    NM.In n inits ->
+    In s (succs n) ->
+    trans n res!!n <= res!!s.
+  Proof.
+    unfold fixpoint; intros. pattern res. 
+    eapply Iter.iter_prop with 
+      (step:=step) (P:=state_invar) (a:=make_init_state); eauto.
+    intros a Ha.
+    unfold step. destruct (wlist a) eqn:Heql. 
+    specialize (Ha n). destruct Ha. 
+      auto. rewrite Heql in *. contradiction. auto.
+
+    eapply step_state_invar. apply Ha. 
+    unfold step. rewrite Heql. auto.
+
+    left. simpl. apply in_map_iff.
+    pose proof (NMFacts.elements_in_iff inits n0) as [He _].
+    specialize (He H2). destruct He as [e Hine].
+    apply InA_alt in Hine as [y [Heq Hk]]. 
+    inversion Heq; eauto.
+  Qed.
+
+  (* monotonicity *)
+
+  Definition le_nlmap (nl1 nl2: nlmap) : Prop :=
+    forall n, nl1!!n <= nl2!!n.
+
+  Lemma le_nlmap_refl : forall nl, le_nlmap nl nl.
+  Proof. 
+    unfold le_nlmap. reflexivity. 
+  Qed.
+  
+  Instance le_nlmap_trans : Transitive le_nlmap.
+    unfold Transitive, le_nlmap; intros. transitivity y !! n; auto.
+  Qed.
+
+  Hint Resolve L.le_join_l L.le_join_r.
+    (* L.eq_equiv L.le_preorder L.le_poset L.eq_le_reflexive. *)
+    (* Saw this in Relation_Definitions but it doesn't appear to work? *)
+
+  Lemma prop_succ_le_nlmap: forall st out n,
+    le_nlmap st.(lmap) (prop_succ out st n).(lmap).
+  Proof.
+    unfold le_nlmap, prop_succ; intros.
+    destruct (L.eq_dec _ _). reflexivity.
+    simpl. destruct (N.eq_dec n n0).
+      subst. rewrite find_default_eq; auto. 
+      rewrite find_default_neq; auto. reflexivity.
+  Qed.
+
+  Lemma step_le_nlmap: forall st st',
+    inr st' = step st ->
+    le_nlmap st.(lmap) st'.(lmap).
+  Proof.
+    unfold step; intros. destruct (wlist st). 
+    discriminate. injection H. intro Heqs.
+    pattern st'. eapply fold_left_1.
+    intros. transitivity (lmap a). 
+      assumption. apply prop_succ_le_nlmap.
+    apply Heqs. apply le_nlmap_refl.
+  Qed.
+    
+  Lemma fixpoint_entry : forall res n,
+    fixpoint = Some res -> inits!!n <= res!!n.
+  Proof.
+    unfold fixpoint. intros. pattern res.
+    eapply Iter.iter_prop with (step:=step). intros.
+    destruct (step a) eqn:Hstep. 
+    unfold step in Hstep. destruct (wlist a); try discriminate.
+    injection Hstep. intro; subst t. apply H0. 
+    simpl in *. transitivity (lmap a)!!n. auto. 
+    apply step_le_nlmap. auto. 
+    change inits with (lmap make_init_state).
+    cbv beta. reflexivity. apply H.
+  Qed.
+
+  Lemma fixpoint_invariant : forall
+    (P: N.t -> L.t -> Prop)
+    (Pinits: forall n, P n inits!!n)
+    (Ptrans: forall n ln s ls,
+      In s (succs n) -> 
+      P n ln -> P s ls -> P s (L.join ls (trans n ln))),
+    forall res n, fixpoint = Some res -> P n res!!n.
+  Proof.
+    intros until 2.
+    unfold fixpoint. intros. pattern res. 
+    eapply Iter.iter_prop with (step:=step); eauto.
+
+    intro. destruct (step a) eqn:Hstep.
+    
+    (* last step  Q implies P *)
+    unfold step in Hstep. destruct (wlist a); try discriminate.
+    instantiate (1:=fun s => forall n, P n s.(lmap)!!n).
+    injection Hstep. intro; subst t. intros; auto.
+
+    (* P preserved across step *)
+    simpl. intros. unfold step in Hstep.
+    destruct (wlist a); try discriminate.
+    injection Hstep; clear Hstep; intro Heqs.
+    
+    pattern s. eapply fold_left_1 with (f:=prop_succ _); eauto.
+    intros. unfold prop_succ. 
+    destruct (L.eq_dec _ _); simpl; auto.
+    destruct (N.eq_dec b n0).
+    rewrite find_default_eq; auto. 
+      subst b. apply Ptrans; auto. 
+    rewrite find_default_neq; auto.
+    auto.
+  Qed.
+
+  End KILDALL.
+
+End ForwardSolver.
+
+  
