src/vminus/LtacDebug.v
@@ -1,0 +1,7 @@
+Require Import String.
+Open Scope string_scope.
+
+(* print list of args to the *trace* buffer in proof general *)
+Tactic Notation "ltrace" constr_list(cl) := idtac "<ltrace>" cl "</ltrace>".
+
+
