src/vminus/Maps.v
@@ -1,0 +1,197 @@
+(* -------------------------------------------------------------------------- *
+ *                     Vellvm - the Verified LLVM project                     *
+ *                                                                            *
+ *     Copyright (c) 2017 Steve Zdancewic <stevez@cis.upenn.edu>              *
+ *                                                                            *
+ *   This file is distributed under the terms of the GNU General Public       *
+ *   License as published by the Free Software Foundation, either version     *
+ *   3 of the License, or (at your option) any later version.                 *
+ ---------------------------------------------------------------------------- *)
+
+
+Require Import Equalities List.
+Import ListNotations.
+
+Set Implicit Arguments.
+
+Module Type Map (K:UsualDecidableType).
+
+Section withv.
+Variable V : Type.
+
+Parameter t : Type -> Type.
+Parameter empty : t V.
+Parameter get : t V -> K.t -> option V.
+Parameter set : t V -> K.t -> V -> t V.
+Parameter rem : t V -> K.t -> t V.
+Parameter dom : t V -> list K.t.
+Parameter forallb2 : (K.t -> V -> bool) -> t V -> bool.
+
+
+Axiom update_eq : forall v k1 k2 m, k2 = k1 -> get (set m k1 v) k2 = Some v.
+Axiom update_neq : forall v k1 k2 m, k2 <> k1 -> get (set m k1 v) k2 = get m k2.
+Axiom get_in_dom : forall m k v, get m k = Some v -> In k (dom m).
+Axiom dom_in_get : forall m k, In k (dom m) -> exists v, get m k = Some v.
+Axiom get_forallb2 : forall m f,
+                       (forall k v, get m k = Some v -> f k v = true) 
+                       <-> forallb2 f m = true.
+End withv.
+
+End Map.
+
+
+Module ListMap (K:UsualDecidableType) <: Map K.
+
+Section withv.
+Variable V : Type.
+
+Definition t := list (K.t * V).
+
+Definition empty : t := [].
+
+Fixpoint get m k : option V := 
+  match m with
+    | [] => None
+    | (k', v) :: m' => if K.eq_dec k k'
+                       then Some v
+                       else get m' k
+  end.
+
+Definition set (m:t) (k:K.t) (v:V) : t :=
+  (k, v) :: m.
+
+
+Fixpoint rem (m:t) (k:K.t) : t :=
+  match m with
+    | [] => []
+    | (k', v) :: m' => if K.eq_dec k k'
+                       then rem m' k
+                       else (k', v) :: rem m' k
+  end.
+
+Fixpoint dom (m:t) : list K.t :=
+  match m with
+    | [] => []
+    | (k', v) :: m' => k' :: dom m'
+  end.
+
+Fixpoint forallb2' (f:K.t -> V -> bool) (m:t) (d:list K.t) : bool :=
+     match d with
+       | [] => true
+       | k :: d' => match get m k with
+                      | None => false
+                      | Some v => f k v && forallb2' f m d'
+                    end
+     end.  
+
+Definition forallb2 (f:K.t -> V -> bool) (m:t) : bool :=
+  forallb2' f m (dom m).
+
+
+Lemma update_eq : forall v k1 k2 m,
+
+    k2 = k1 -> get (set m k1 v) k2 = Some v.
+Proof.
+  intros; simpl. destruct (K.eq_dec _ _); intuition.
+Qed.
+
+
+Lemma update_neq : forall v k1 k2 m,
+  k2 <> k1 -> get (set m k1 v) k2 = get m k2.
+Proof.
+  intros; simpl. destruct (K.eq_dec _ _); intuition.
+Qed.
+
+Lemma get_in_dom : forall m k v,
+  get m k = Some v -> In k (dom m).
+Proof.
+  induction m; intros k v. inversion 1.
+  destruct a as [k' v']; simpl in *. intros. destruct (K.eq_dec k k'); intuition eauto. 
+Qed.
+
+Lemma dom_in_get : forall m k,
+  In k (dom m) -> exists v, get m k = Some v.
+Proof.
+  induction m. inversion 1.
+  destruct a as [k' v']; simpl in *. 
+  intro k. destruct (K.eq_dec k k') as [|Heq]; intros. intuition eauto.
+  inversion H; eauto; contradict Heq; auto.
+Qed.
+
+Lemma get_forallb2' : forall m f P,
+  (forall k v, P k v <-> f k v = true) ->
+  ((forall k v, get m k = Some v -> P k v)
+   <-> forallb2 f m = true).
+Proof.
+  intros until 0. intro Hpf. unfold forallb2.
+  split; intros.
+
+  - (* Case "->". *)
+  pose proof (dom_in_get m) as Hd.
+  set (d := dom m) in *. clearbody d.
+
+  induction d. reflexivity. simpl. 
+  destruct (get m a) eqn:Hget.
+  rewrite IHd; auto. assert (f a v = true).
+  apply Hpf. eapply H; eauto. rewrite H0. simpl. reflexivity.
+  intros. apply Hd. simpl. right. auto.
+  
+  ecase (Hd a) as [v Hv]; try (left; auto). 
+  rewrite Hv in Hget. inversion Hget.
+
+  - (* Case "<-". *)
+  pose proof (get_in_dom m _ H0) as Hd.
+  set (d:=dom m) in *. clearbody d.
+
+  induction d. inversion Hd.
+  simpl in H.
+  destruct (K.eq_dec a k). subst a. rewrite H0 in H.
+  apply Hpf; auto. destruct (f k v); auto. 
+  apply IHd. destruct (get m a); try solve [inversion H].
+  destruct (f a v0).
+  destruct (forallb2' f m d); auto.
+  destruct (forallb2' f m d); auto.
+  inversion Hd; intuition.
+Qed.  
+
+
+Lemma get_forallb2 : forall m f,
+  (forall k v, get m k = Some v -> f k v = true) 
+  <-> 
+  forallb2 f m = true.
+Proof.
+  intros. unfold forallb2.
+  split; intros.
+
+  - (* Case "->". *)
+  pose proof (dom_in_get m) as Hd.
+  set (d := dom m) in *. clearbody d.
+
+  induction d. reflexivity. simpl. 
+  destruct (get m a) eqn:Hget.
+  rewrite H; auto. rewrite IHd; auto. intros.
+  apply Hd. simpl. right; auto.
+  
+  ecase (Hd a) as [v Hv]; try (left; auto). 
+  rewrite Hv in Hget. inversion Hget.
+
+  - (* Case "<-". *)
+  pose proof (get_in_dom m _ H0) as Hd.
+  set (d:=dom m) in *. clearbody d.
+
+  induction d. inversion Hd.
+  simpl in H.
+  destruct (K.eq_dec a k). subst a. rewrite H0 in H.
+  destruct (f k v); auto.
+  apply IHd.
+  destruct (get m a); try solve [inversion H].
+  destruct (forallb2' f m d); auto.
+  destruct (f a v0); auto.
+  inversion Hd; intuition.
+Qed.  
+
+End withv.
+
+End ListMap.
+
+
