src/vminus/Sequences.v
@@ -1,0 +1,316 @@
+(* 
+  Acknowledgements:  
+  This file is taken from the compiler verification development created by 
+
+    Xavier Leroy, INRIA Paris-Rocquencourt                    
+
+  and available at: http://gallium.inria.fr/~xleroy/courses/Eugene-2012/
+*)
+
+
+(** A library of relation operators defining sequences of transitions
+  and useful properties about them. *)
+
+Set Implicit Arguments.
+
+Section SEQUENCES.
+
+Variable A: Type.                 (**r the type of states *)
+Variable R: A -> A -> Prop.       (**r the transition relation, from one state to the next *)
+
+(** ** Finite sequences of transitions *)
+
+(** Zero, one or several transitions: reflexive, transitive closure of [R]. *)
+
+Inductive star: A -> A -> Prop :=
+  | star_refl: forall a,
+      star a a
+  | star_step: forall a b c,
+      R a b -> star b c -> star a c.
+
+Lemma star_one:
+  forall (a b: A), R a b -> star a b.
+Proof.
+  intros. econstructor; eauto. constructor.
+Qed.
+
+Lemma star_trans:
+  forall (a b: A), star a b -> forall c, star b c -> star a c.
+Proof.
+  induction 1; intros. auto. econstructor; eauto.
+Qed.
+
+(** One or several transitions: transitive closure of [R]. *)
+
+Inductive plus: A -> A -> Prop :=
+  | plus_left: forall a b c,
+      R a b -> star b c -> plus a c.
+
+Lemma plus_one:
+  forall a b, R a b -> plus a b.
+Proof.
+  intros. apply plus_left with b. auto. apply star_refl.
+Qed.
+
+Lemma plus_star:
+  forall a b,
+  plus a b -> star a b.
+Proof.
+  intros. inversion H. eapply star_step; eauto. 
+Qed.
+
+Lemma plus_star_trans:
+  forall a b c, plus a b -> star b c -> plus a c.
+Proof.
+  intros. inversion H. eapply plus_left; eauto. eapply star_trans; eauto.
+Qed.
+
+Lemma plus_star_trans':
+  forall a b c, star a b -> plus b c -> plus a c.
+Proof.
+  intros. inversion H. auto. apply plus_star in H0. 
+  eapply plus_left. eauto. eapply star_trans; eauto.
+Qed.
+
+
+Lemma star_plus_trans:
+  forall a b c, star a b -> plus b c -> plus a c.
+Proof.
+  intros. inversion H0. inversion H. econstructor; eauto.
+  econstructor; eauto. eapply star_trans; eauto. econstructor; eauto. 
+Qed.
+
+Lemma plus_right:
+  forall a b c, star a b -> R b c -> plus a c.
+Proof.
+  intros. eapply star_plus_trans; eauto. apply plus_one; auto.
+Qed.
+
+(** ** Infinite sequences of transitions *)
+
+(** It is easy to characterize the fact that all transition sequences starting
+  from a state [a] are infinite: it suffices to say that any finite sequence
+  starting from [a] can always be extended by one more transition. *)
+
+Definition all_seq_inf (a: A) : Prop :=
+  forall b, star a b -> exists c, R b c.
+
+(** However, this is not the notion we are trying to characterize: that, starting
+  from [a], there exists one infinite sequence of transitions
+  [a --> a1 --> a2 --> ... -> aN -> ...].
+
+  Indeed, consider [A = nat] and [R] such that [R 0 0] and [R 0 1].  
+  [all_seq_inf 0] does not hold, because a sequence [0 -->* 1] cannot be extended.
+  Yet, [R] admits an infinite sequence, namely [0 --> 0 --> ...].  
+
+  Another attempt would be to represent the sequence of states 
+  [a0 --> a1 --> a2 --> ... -> aN -> ...] explicitly, as a function 
+  [f: nat -> A] such that [f i] is the [i]-th state [ai] of the sequence. *)
+
+Definition infseq_with_function (a: A) : Prop :=
+  exists f: nat -> A, f 0 = a /\ forall i, R (f i) (f (1 + i)).
+
+(** This is a correct characterization of the existence of an infinite sequence
+  of reductions.  However, it is very inconvenient to work with this definition
+  in Coq's constructive logic: in most use cases, the function [f] is not
+  computable and therefore cannot be defined in Coq.  *)
+
+(** To obtain a practical definition of infinite sequences, we use the following
+  coinductive definition of the predicate [infseq a]. *)
+
+CoInductive infseq: A -> Prop :=
+  | infseq_step: forall a b,
+      R a b -> infseq b -> infseq a.
+
+(** An inductive predicate such as [star a b] holds iff there exists a finite
+  derivation of the conclusion [star a b] that uses the constructors
+  [star_refl] and [star_step] a finite number of times.
+
+  A coinductive predicate is similar, but holds iff there exists a finite
+  OR INFINITE derivation of the conclusion that uses the constructors
+  of the predicate a finite OR INFINITE number of times.
+
+  In other words, an inductive predicate is a smallest fixpoint: the smallest predicate
+  that satisfies its constructors; a coinductive predicate is a greatest fixpoint:
+  the largest predicate that satisfies its constructors.
+
+  The [infseq] predicate above must be defined coinductively.  Indeed, if
+  we define it inductively, the predicate would be empty (always false),
+  since there are no base cases!  
+
+  Coq provides some primitive support for constructing infinite derivations
+  of facts such as [infseq a].  Such constructions are proofs by coinduction.
+  For example, we can prove the following: *)
+
+Remark cycle_infseq:
+  forall a, R a a -> infseq a.
+Proof.
+  intros. cofix COINDHYP. apply infseq_step with a. auto. apply COINDHYP.
+Qed.
+
+(** This style of proof by coinduction, using the [cofix] tactic, is effective
+  but can run into limitations of Coq's proof engine (the so-called 
+  "guard condition").  However, we can derive more conventional
+  coinduction principles that are often easier to use. *)
+
+(** Consider a set [X] of states [A], that is, a predicate [X: A -> Prop].
+  Assume that for every [a] in [X], we can make one [R] transition to a [b]
+  that is still in [X].  Then, starting from [a] in [X], we can transition
+  to some [a1] in [X], then to some [a2] still in [X], then... It is clear
+  that we are just building an infinite sequence of transitions starting from
+  [a]. Therefore [infseq a] should hold.  Let's prove this! *)
+
+Lemma infseq_coinduction_principle:
+  forall (X: A -> Prop),
+  (forall a, X a -> exists b, R a b /\ X b) ->
+  forall a, X a -> infseq a.
+Proof.
+  intros X P. cofix COINDHYP; intros.
+  destruct (P a H) as [b [U V]]. apply infseq_step with b; auto. 
+Qed.
+
+(** An even more useful variant of this coinduction principle considers a
+  set [X] where for every [a] in [X], we can make one *or several* transitions
+  to reach a [b] in [X].  *)
+
+Lemma infseq_coinduction_principle_2:
+  forall (X: A -> Prop),
+  (forall a, X a -> exists b, plus a b /\ X b) ->
+  forall a, X a -> infseq a.
+Proof.
+  intros.
+  apply infseq_coinduction_principle with
+    (X := fun a => exists b, star a b /\ X b).
+  intros. 
+  destruct H1 as [b [STAR Xb]]. inversion STAR; subst.
+  destruct (H b Xb) as [c [PLUS Xc]]. inversion PLUS; subst.
+  exists b0; split. auto. exists c; auto. 
+  exists b0; split. auto. exists b; auto.
+
+  exists a; split. apply star_refl. auto.
+Qed.
+
+(** Here is an example of use of [infseq_coinduction_principle]:
+  if all finite transition sequences starting at [a] can be extended,
+  [infseq a] holds. *)
+
+Lemma infseq_if_all_seq_inf:
+  forall a, all_seq_inf a -> infseq a.
+Proof.
+  apply infseq_coinduction_principle.
+  intros. destruct (H a) as [b Rb]. constructor. 
+  exists b; split; auto. 
+  unfold all_seq_inf; intros. apply H. apply star_step with b; auto.
+Qed.
+
+(** Likewise, the function-based characterization [infseq_with_function]
+  implies [infseq]. *)
+
+Lemma infseq_from_function:
+  forall a, infseq_with_function a -> infseq a.
+Proof.
+  apply infseq_coinduction_principle.
+  intros. destruct H as [f [P Q]].
+  exists (f 1); split.
+  subst a. apply Q. 
+  exists (fun n => f (1 + n)); split. auto. intros. apply Q.
+Qed.
+ 
+(** Consider the transition sequences starting at state [a].
+  They can be infinite, or they can be finite: after a number of transitions,
+  we reach a state from with no transition is possible.  It is intuitively
+  obvious that at least one of the two cases must hold. 
+
+  It is however impossible to prove this fact in Coq's constructive logic.
+  Indeed, a constructive proof would be isomorphic (by the Curry-Howard isomorphism)
+  to a terminating function that solves Turing's halting problem!
+
+  To prove this fact, we must enrich Coq with axioms from classical logic,
+  namely the axiom of excluded middle: for all propositions [P],
+  either [P] or [~P] hold.  The Coq standard library provides such axioms
+  in the module named [Classical], which we now import. *)
+
+Require Import Classical.
+
+Definition irred (a: A) : Prop := forall b, ~(R a b).
+
+Lemma infseq_or_finseq:
+  forall a, infseq a \/ exists b, star a b /\ irred b.
+Proof.
+  intros.
+  destruct (classic (forall b, star a b -> exists c, R b c)).
+  left. apply infseq_if_all_seq_inf; auto.
+  right.
+  generalize (not_all_ex_not _ _ H). intros [b P].
+  generalize (imply_to_and _ _ P). intros [U V].
+  exists b; split. auto.
+  red; intros; red; intros. elim V. exists b0; auto.
+Qed.
+
+(** ** Determinism properties for functional transition relations. *)
+
+(** A transition relation is functional if every state can transition to at most
+  one other state. *)
+
+Hypothesis R_functional:
+  forall a b c, R a b -> R a c -> b = c.
+
+(** Uniqueness of finite transition sequences. *)
+
+Lemma star_star_inv:
+  forall a b, star a b -> forall c, star a c -> star b c \/ star c b.
+Proof.
+  induction 1; intros.
+  auto.
+  inversion H1; subst. right. eapply star_step; eauto. 
+  assert (b = b0). eapply R_functional; eauto. subst b0. 
+  apply IHstar; auto.
+Qed.
+
+Lemma finseq_unique:
+  forall a b b',
+  star a b -> irred b ->
+  star a b' -> irred b' ->
+  b = b'.
+Proof.
+  intros. destruct (star_star_inv H H1).
+  inversion H3; subst. auto. elim (H0 _ H4).
+  inversion H3; subst. auto. elim (H2 _ H4).
+Qed.
+
+(** A state cannot both diverge and terminate on an irreducible state. *)
+
+Lemma infseq_star_inv:
+  forall a b, star a b -> infseq a -> infseq b.
+Proof.
+  induction 1; intros. auto. 
+  inversion H1; subst. assert (b = b0). eapply R_functional; eauto. subst b0.
+  apply IHstar. auto.
+Qed.
+
+Lemma infseq_finseq_excl:
+  forall a b,
+  star a b -> irred b -> infseq a -> False.
+Proof.
+  intros. 
+  assert (infseq b). eapply infseq_star_inv; eauto. 
+  inversion H2. elim (H0 b0); auto. 
+Qed.
+
+(** If there exists an infinite sequence of transitions from [a],
+  all sequences of transitions arising from [a] are infinite. *)
+
+Lemma infseq_all_seq_inf:
+  forall a, infseq a -> all_seq_inf a.
+Proof.
+  intros. unfold all_seq_inf. intros. 
+  assert (infseq b). eapply infseq_star_inv; eauto. 
+  inversion H1. subst. exists b0; auto.
+Qed.
+
+End SEQUENCES.
+
+
+  
+
+
