src/vminus/Stmon.v
@@ -1,0 +1,92 @@
+(* -------------------------------------------------------------------------- *
+ *                     Vellvm - the Verified LLVM project                     *
+ *                                                                            *
+ *     Copyright (c) 2017 Steve Zdancewic <stevez@cis.upenn.edu>              *
+ *                                                                            *
+ *   This file is distributed under the terms of the GNU General Public       *
+ *   License as published by the Free Software Foundation, either version     *
+ *   3 of the License, or (at your option) any later version.                 *
+ ---------------------------------------------------------------------------- *)
+
+
+Set Implicit Arguments.
+Set Maximal Implicit Insertion.
+
+Section STMON.
+
+  Variable (S : Type).
+
+  Definition stmon (A:Type) : Type := S -> (S * A).
+
+  Definition ret (A:Type) (a:A) : stmon A := fun s => (s, a).
+
+  Definition bind (A B:Type) (m:stmon A) (f:A -> stmon B) : (stmon B) :=
+    fun s => let (s', a) := m s in f a s'.
+
+  Definition bind2 (A B C:Type) (f:stmon (A * B)) (g:A -> B -> stmon C) : stmon C :=
+    fun s => let '(s', (a, b)) := f s in g a b s'.
+
+  Definition stget : stmon S := 
+    fun s => (s, s).
+
+  Definition stput (s:S) : stmon unit := 
+    fun _ => (s, tt).
+
+  Definition stmod (f:S -> S) : stmon unit :=
+    fun s => (f s, tt).
+
+  (* Definition strun (A:Type) (ma:stmon A) (s:S) : (S * A) := *)
+  (*   ma s. *)
+
+  Definition steval (A:Type) (ma:stmon A) (s:S) : A :=
+    snd (ma s).
+
+  Definition stexec (A:Type) (ma:stmon A) (s:S) : S :=
+    fst (ma s).
+
+  (* Global Arguments steval _ _ _ /. *)
+  (* Global Arguments stexec _ _ _ /. *)
+
+  Definition stlift (A:Type) (R:S -> S -> Prop) : stmon A -> Prop :=
+    fun ma => forall s, R s (fst (ma s)).
+
+  Require Import FunctionalExtensionality.
+
+  Lemma stmon_left_id : forall A B (a:A) (f: A -> stmon B),
+    bind (ret a) f = f a.
+  Proof. 
+    intros. unfold bind, ret. 
+    change (f a) with (fun s => f a s) at 2; auto.
+  Qed.
+
+  Lemma stmon_right_id : forall A (a:A) (ma:stmon A),
+    bind ma ret = ma.
+  Proof. 
+    intros. extensionality s. unfold bind, ret.
+    destruct (ma s); reflexivity.
+  Qed.
+
+  Lemma stmon_assoc : 
+    forall A B C (m:stmon A) (f:A -> stmon B) (g:B -> stmon C),
+    bind m (fun a => bind (f a) g) = bind (bind m f) g.
+  Proof.
+    intros. extensionality s. unfold bind.
+    destruct (m s); reflexivity.
+  Qed.
+
+End STMON.
+
+Infix ">>=" := bind (at level 100, no associativity) : stmon_scope.
+Infix ">>=2" := bind2 (at level 100, no associativity) : stmon_scope.
+
+Notation "m '>>>' k" := (bind m (fun _:unit => k))
+  (at level 100, right associativity) : stmon_scope.
+
+Notation "'do' X <- A ; B" := (bind A (fun X => B))
+  (at level 200, X ident, A at level 100, B at level 200) : stmon_scope.
+
+Notation "'do' ( X , Y ) <- A ; B" := (bind2 A (fun X Y => B))
+  (at level 200, X ident, Y ident, A at level 100, B at level 200, 
+  format "'do'  ( X ,  Y )  <-  A  ;  B") : stmon_scope.
+
+Delimit Scope stmon_scope with stmon.
