src/vminus/Vminus.v
@@ -1,0 +1,1173 @@
+(** * Vminus: A Simple SSA Intermediate Representation *)
+
+(** FULL: This file defines the syntax and semantics for Vminus, an
+    intermediate representation that is intended to capture the
+    essence of LLVM's IR.  In particular, this language represents
+    code as a _control flow graph_ whose blocks contain instructions
+    in _static single assignment_ form.  This means that each
+    instruction _defines_ (at most) one local identifier and that
+    those identifiers are _immutable_.  To make this work in practice,
+    SSA representations introduce the notation of _phi functions_,
+    whose value is determined by the run-time control flow of the
+    program.
+
+    To support mutable state, Vminus also has Imp-style global
+    identifiers.
+*)
+
+(** TERSE: Vminus is a highly simplified model of the LLVM IR that 
+    features:
+    - programs represented as _control flow graphs_ 
+    - SSA _single static assignment_ form
+      - uniquely defined _immutable local identifiers_ 
+      - _phi functions_ 
+    - Mutable, global state with [load] and [store] operations, as in IMP.
+*)
+
+Require Import Arith List.
+Import ListNotations.
+Require Import Atom Dom Env Imp Util.
+
+(* ####################################################### *)
+(** ** Vminus Overview *)
+
+(** See the course slides for a high-level overview of the concepts of
+    the Vminus IR.
+
+    The remainder of this section defines the syntax, operational
+    semantics, and typing (well-formedness) rules for Vminus in Coq.  
+*)
+
+
+(* ####################################################### *)
+(** *** Vminus labels, identifiers, and addresses.  *)
+
+
+(** Basic block labels *)
+
+Module Lbl : ATOM := Atom.
+Notation lbl := Lbl.t.
+
+(** Local unique identifiers *)
+
+Module Uid : ATOM := Atom.
+Notation uid := Uid.t.
+
+(** Mutable (integer) addresses *)
+
+(* HIDE: Note, cannot ascribe Var : ATOM because var fails to
+   be considered equivalent to Imp.id  *)
+Module Addr := Atom. 
+Notation addr := Addr.t.
+
+(** *** Values and Binary Operations *)
+
+(** Values are just local identifiers or natural numbers *)
+
+Inductive val : Set :=
+ | val_uid  : uid -> val
+ | val_nat : nat -> val.
+
+(** All Vminus operations are binary arithmetic forms.  There are no
+    unary operations, nor are there assembly-language-like [move]
+    instructions.
+*)
+
+Inductive bop : Set := 
+ | bop_add 
+ | bop_sub 
+ | bop_mul
+ | bop_eq  
+ | bop_le  
+ | bop_and.
+
+(** *** Basic block terminators *)
+
+(** Each basic block is a sequence of commands (defined next) ending
+    in a _terminator_, which is just a control flow operation.  
+    Terminators cannot appear in the middle of a well-formed basic block.   
+*)
+
+Inductive tmn : Set :=
+| tmn_jmp : lbl -> tmn                  (* unconditional jump *)
+| tmn_cbr : val -> lbl -> lbl -> tmn    (* conditional branch *)
+| tmn_ret : tmn.                        (* return *)
+
+
+(** *** Commands *)
+
+(** Vminus has only a few commands: binary operations, phi nodes,
+terminators, and [load] and [store] operations. *)
+
+(** Each [phiarg] associates a value with a predessor block. *)
+
+Definition phiarg := (lbl * val)%type.
+
+(** Vminus Commands *)
+
+Inductive cmd : Set :=
+| cmd_bop   : bop -> val -> val -> cmd
+| cmd_phi   : list phiarg -> cmd
+| cmd_tmn   : tmn -> cmd
+| cmd_load  : addr -> cmd
+| cmd_store : addr -> val -> cmd.
+
+(** An instruction associates a unique local identifier with one of the
+    above commands. *)
+
+Definition insn := (uid * cmd)%type.
+
+
+(* ####################################################### *)
+
+(** *** Useful information about instructions *)
+
+Definition insn_uses (i:insn) : list val :=
+(* FOLD *)
+  match i with
+    | (_, cmd_bop _ v1 v2) => [v1; v2]
+    | (_, cmd_tmn (tmn_cbr v _ _)) => [v]
+    | (_, cmd_store _ v) => [v]
+(* TODO:     | (_, cmd_phi pas) => map (@snd _ _) pas *)
+    | _ => []
+  end.
+(* /FOLD *)
+
+Definition insn_lbls (i:insn) : list lbl :=
+(* FOLD *)
+  match i with 
+    | (_, cmd_tmn (tmn_jmp l)) => [l]
+    | (_, cmd_tmn (tmn_cbr _ l1 l2)) => [l1; l2]
+    | _ => []
+  end.
+(* /FOLD *)
+
+Definition insn_phis (i:insn) : list phiarg :=
+(* FOLD *)
+  match i with
+    | (_, cmd_phi pas) => pas
+    | _ => []
+  end.
+(* /FOLD *)
+
+Definition is_tmn (i:insn) : Prop := 
+(* FOLD *)
+  match i with (_, cmd_tmn _) => True | _ => False end.
+(* /FOLD *)
+
+Definition is_phi (i:insn) : Prop := 
+(* FOLD *)
+  match i with (_, cmd_phi _) => True | _ => False end.
+(* /FOLD *)
+
+Definition defs_uid (i:insn) : Prop :=
+(* FOLD *)
+  match i with
+    | (_, cmd_tmn _) | (_, cmd_store _ _) => False | _ => True
+  end.
+(* /FOLD *)
+
+(** ** Program points *)
+
+(** FULL: Vminus programs are structured into _control-flow graphs_
+    (CFG), which, conceptually, are graphs whose _nodes_ are basic
+    blocks and whose _edges_ are determined by the control structure
+    of the program.  A block [b1] terminated by a jump to [b2]
+    requires and edge from [b1] to [b2] in the CFG.  Similarly a block
+    terminated by a branch to either [b2] or [b3] has two successors
+    edges.
+
+    To characterize this structure abstractly, we define a notion of
+    _program point_ [pc], which is a location of an instruction in the
+    control-flow graph.  A [pc] is given by a block label and offset.
+    The program points within a single block increase by offset order;
+    program points in two different blocks are connected by the
+    control structure as determined above.
+*)
+(** TERSE: Vminus programs are _control-flow graphs_ that have:
+    - _Program points_ [pc] given by block labels and an offset.
+    - Successor edges determined by offset within a block and the control flow operations between blocks. 
+*)   
+
+(** Program points (a.k.a. "program counters"). *)
+
+Definition pc := (lbl * nat)%type.
+Definition lbl_of : pc -> lbl       := @fst _ _.
+
+(** Increment a [pc] _within_ a block. *)
+
+Definition incr_pc (p:pc) : pc :=
+  let (l, n) := p in (l, S n).
+
+(** (Total) Ordering on [pc]s within the same block *)
+
+Inductive le_pc : pc -> pc -> Prop :=
+| let_pc_intro : forall l n1 n2,
+    n1 <= n2 -> le_pc (l, n1) (l, n2).
+
+Definition lt_pc (p1 p2:pc) : Prop :=
+  le_pc p1 (incr_pc p2).
+
+(** The entry point of a block is offset [0]. *)
+
+Definition block_entry (l:lbl) : pc := (l, 0).
+Definition entry_of_pc (p:pc)  : pc := block_entry (fst p).
+
+(** ** Well-formed Control-flow Graphs *)
+
+(** FULL: Given the abstract characterization of program points, we need to
+    relate them to the control-flow instructions of the program's CFG.
+    We do this via a collection of well-formedness predicates that
+    ensure that each program point maps to a single instruction and
+    that the instruction defines a unique local identifier.  (Thus
+    satisfying the 'single static assignment' part of the SSA
+    representation.)
+ *)
+
+(** TERSE:
+    - Relate program points to the control-flow instructions.
+    - Each pc maps to a single instruction.
+    - Each instruction defines a unique uid.
+*)
+
+(** A module signature defining well-formed control-flow graphs. *)
+
+Module Type CFG.
+  Parameter t : Type.
+  Local Notation cfg := t.
+
+(** *** Basic parameters of the model *)
+
+  (** Well-formed control-flow-graphs. *)
+
+  Parameter wf_cfg : cfg -> Prop.
+
+  (** Well-formed program points. *)
+
+  Parameter wf_pc : cfg -> pc -> Prop.
+
+  (** *** *)
+
+  (** The entry block of the control-flow graph. *)
+
+  Parameter entry_block : cfg -> lbl.
+
+  (** Is the program point a block terminator? *)
+
+  Parameter tmn_pc : cfg -> pc -> Prop.
+
+  (** *** Program point properties *)
+
+  (** Program points are associated with unique instructions. *)
+
+  Parameter insn_at_pc : cfg -> pc -> insn -> Prop.
+
+  Definition uid_at_pc (g:cfg) (p:pc) (uid:uid) : Prop :=
+    exists c, insn_at_pc g p (uid, c).
+
+  Axiom insn_at_pc_func : forall g, wf_cfg g ->
+    functional (insn_at_pc g).
+
+  Axiom uid_at_pc_inj : forall g, wf_cfg g ->
+    injective (uid_at_pc g).
+
+  Axiom wf_pc_insn : forall g, wf_cfg g ->
+    forall p, wf_pc g p -> exists i, insn_at_pc g p i.
+
+  (** *** Block properties *)
+
+  (** There is an instruction in the entry block. *)
+
+  Axiom wf_entry : forall g, wf_cfg g ->
+    wf_pc g (block_entry (entry_block g)).
+
+  (** Every block has a terminator. *)
+
+  Axiom wf_pc_tmn : forall g, wf_cfg g ->
+    forall p, wf_pc g p -> exists p', tmn_pc g p' /\ le_pc p p'.
+
+  (** There are no "gaps" in the pc labels. *)
+
+  Axiom wf_pc_le_tmn : forall g, wf_cfg g ->
+    forall p', tmn_pc g p' -> forall p, le_pc p p' -> wf_pc g p.
+
+End CFG.
+
+(** ** Vminus Operational Semantics *)
+Module Make (Import Cfg:CFG).
+
+Module Opsem.
+
+  (** *** The state of a Vminus program: *)
+
+  Module Locals := Make_Env(Uid).
+  Module Memory := Make_Env(Addr).
+  Notation loc := (Locals.t (option nat)).
+  Notation mem := (Memory.t nat).
+  Notation update := Locals.update.
+
+  Record state := mkst { st_mem  : mem
+                       ; st_pc   : pc
+                       ; st_loc  : loc
+                       ; st_ppc  : pc     (* predecessor pc *)
+                       ; st_ploc : loc    (* predecessor locals *) 
+                       }.
+
+  (** *** Evaluating values. *)
+
+  (** Simply look up the uid in the locals state. (May fail!) *)
+  
+  Definition eval_val (loc:loc) (v:val) : option nat :=
+    match v with
+      | val_nat n => Some n
+      | val_uid i => loc i
+    end.
+
+  (** *** Evaluating binary operations. *)
+
+  Definition b2n (b:bool) := if b then 1 else 0.
+  Definition n2b (n:nat) := if n then false else true.
+
+  Definition bop_denote (bop:bop) : nat -> nat -> nat :=
+    match bop with
+      | bop_add => plus
+      | bop_sub => minus
+      | bop_mul => mult
+      | bop_eq => fun n m => b2n (beq_nat n m)
+      | bop_le => fun n m => b2n (leb n m)
+      | bop_and => fun n m => b2n (n2b n && n2b m)
+    end.
+
+  Definition eval_bop (loc:loc) (bop:bop) (v1 v2:val) : option nat :=
+    match eval_val loc v1, eval_val loc v2 with
+      | Some n1, Some n2 => Some (bop_denote bop n1 n2) 
+      | _, _ => None
+    end.
+
+  (** *** Phi nodes *)
+  (** Look up the predecessor label in the phi arg list. *)
+
+  Definition eval_phi (loc:loc) (l:lbl) (pas:list phiarg) 
+    : option nat :=
+    match assoc Lbl.eq_dec l pas with
+      | Some v => eval_val loc v
+      | None => None
+    end.
+
+  (** *** Control transfers. *)
+  
+  (** Given the current locals and the terminator, determine
+      the label of the next block to jump to. *)
+
+  Definition eval_tmn (loc:loc) (t:tmn) : option lbl :=
+    match t with
+      | tmn_jmp l => Some l
+      | tmn_cbr v l1 l2 =>
+          match eval_val loc v with
+            | Some n => Some (if n then l2 else l1)
+            | None => None
+          end
+      | _ => None
+    end.
+
+  (** *** Small-step, relational operational semantics *)
+
+  Inductive step (g:Cfg.t) : state -> state -> Prop :=
+
+  | step_bop : forall mem pc loc bop v1 v2 uid n ppc ploc,
+      insn_at_pc g pc (uid, cmd_bop bop v1 v2) ->
+      Some n = eval_bop loc bop v1 v2 ->
+      step g (mkst mem pc loc ppc ploc) 
+             (mkst mem (incr_pc pc) 
+                       (update loc uid (Some n)) ppc ploc)
+
+
+
+
+
+
+
+
+
+
+
+
+  (** Evaluate the right-hand side in the predecessor's 
+     local environment. [lbl_of ppc] is the control-flow 
+     edge that we jumped from. *)
+  | step_phi : forall mem pc loc pas uid n ppc ploc,
+      insn_at_pc g pc (uid, cmd_phi pas) ->
+      Some n = eval_phi ploc (lbl_of ppc) pas ->
+      step g (mkst mem pc loc ppc ploc)
+             (mkst mem (incr_pc pc) 
+                       (update loc uid (Some n)) ppc ploc)
+
+
+
+
+
+
+
+
+
+
+  (** Find the successor block (if any), update the pc. 
+      Record the current pc and locals as the "predecessor" state. *)
+  | step_tmn : forall mem pc l' loc tmn uid ppc ploc, 
+      insn_at_pc g pc (uid, cmd_tmn tmn) ->
+      Some l' = eval_tmn loc tmn ->
+      step g (mkst mem pc loc ppc ploc)
+             (mkst mem (block_entry l') loc pc loc)
+
+
+
+
+
+
+
+
+
+
+  | step_load : forall mem pc loc uid addr ppc ploc,
+      insn_at_pc g pc (uid, cmd_load addr) ->
+      step g (mkst mem pc loc ppc ploc)
+             (mkst mem (incr_pc pc) 
+                       (update loc uid (Some (mem addr))) ppc ploc)
+
+  | step_store : forall mem pc loc uid addr v n ppc ploc,
+      insn_at_pc g pc (uid, cmd_store addr v) ->
+      Some n = eval_val loc v ->
+      step g (mkst mem pc loc ppc ploc)
+             (mkst (Memory.update mem addr n) 
+                   (incr_pc pc) loc ppc ploc).
+  
+
+
+
+ (** Definition of the initial state. *)
+
+  Definition init_state (g:Cfg.t) (m: mem) : state :=
+    (mkst m
+          (block_entry (entry_block g))
+          (Locals.empty None)
+          (block_entry (entry_block g))
+          (Locals.empty None)).
+
+End Opsem.
+
+
+(** ** Typing *)
+(** FULL: The only ways in which a Vminus program can "go wrong" are
+    by accessing a local variable that hasn't been defined or jumping
+    to a label that isn't in the CFG.  Therefore, its typing
+    constraints ensure that each instruction only mentions local
+    identifiers that are in scope according to the domination
+    structure of the control-flow graph and that all mentioned labels
+    are associated with blocks defined in the CFG.  *)
+
+(** TERSE:
+    The type system for Vminus ensures that:
+    - All local variables are defined.
+    - All jump targets are legal.
+*)
+
+Module Typing.
+
+
+  (** *** GRAPH instance for dominance calculation *)
+
+  (** Edge relation *)
+
+  Inductive succ_pc (g:Cfg.t) : pc -> pc -> Prop :=
+  | succ_pc_S : forall p,
+      succ_pc g p (incr_pc p)
+  | succ_pc_J : forall p l i,
+      insn_at_pc g p i ->
+      In l (insn_lbls i) ->
+      succ_pc g p (block_entry l).
+
+  (** Graph of program points *)
+
+  Module PcGraph <: GRAPH.
+    Definition t := Cfg.t.
+    Definition V := pc.
+    Definition entry g := block_entry (entry_block g).
+    Definition Succ := succ_pc.
+    Definition Mem := wf_pc.
+  End PcGraph.
+
+  Module Export Dom := Dom.Spec PcGraph.
+
+  (** *** Definitions for Well-formed SSA programs. *)
+
+  (** FULL: Most of the Vminus instructions define the uid associated
+  with their program point.  Some (like [store] and the [tmn]s)
+  do not. *)
+  (** TERSE: The command at the given [pc] defines uid. *)
+
+  Definition def_at_pc (g:Cfg.t) (p:pc) (uid:uid) : Prop :=
+    exists c, insn_at_pc g p (uid, c) /\ defs_uid (uid, c). 
+
+  (** The definition of [uid] strictly dominates the pc. *)
+ 
+  Definition uid_sdom_pc (g:Cfg.t) (uid:uid) (p:pc) : Prop :=
+    exists p', def_at_pc g p' uid /\ SDom g p' p.
+
+  (** All uses of a [uid] must be strictly dominated by
+      their definitions. *)
+
+  Definition wf_use (g:Cfg.t) (i:insn) (p:pc) : Prop :=
+    forall uid, In (val_uid uid) (insn_uses i) -> uid_sdom_pc g uid p.
+
+  (** All jump targets must be legal block labels. *)
+
+  Definition wf_lbl (g:Cfg.t) (i:insn) : Prop :=
+    forall l, In l (insn_lbls i) -> wf_pc g (block_entry l).
+
+  (** *** Well-formed phi nodes *)
+
+  (**  Consider [ %x = phi [lbl1:v1, ...,lbln:vn] ].  This is well formed
+       when every predecessor block with terminator program point p' 
+       has a label associated with value v.  Moreover, if v is a uid then
+       the definition of the uid strictly dominates p'.
+  *)
+
+  Definition wf_phi_args (g:Cfg.t) (i:insn) (p:pc) : Prop :=
+    forall pred, succ_pc g pred (entry_of_pc p) ->
+      (exists v, In (lbl_of pred, v) (insn_phis i)) /\
+      (forall uid, In (lbl_of pred, val_uid uid) (insn_phis i) -> 
+          uid_sdom_pc g uid pred).
+
+  Definition wf_phi_pred (g:Cfg.t) (i:insn) (p:pc) : Prop :=
+    forall l v, In (l, v) (insn_phis i) ->
+      (exists pred, succ_pc g pred (entry_of_pc p) /\ lbl_of pred = l).
+
+  Definition wf_phi (g:Cfg.t) (i:insn) (p:pc) : Prop :=
+    is_phi i -> wf_phi_args g i p
+             /\ wf_phi_pred g i p
+             /\ insn_phis i <> [].
+
+  (** *** Well-formed instructions *)
+
+  Inductive wf_insn (g:Cfg.t) : insn -> pc -> Prop :=
+  | wf_insn_intro : forall i p,
+      wf_use g i p ->
+      wf_lbl g i ->
+      wf_phi g i p ->
+      wf_insn g i p.
+
+  Inductive wf_prog (g:Cfg.t) : Prop :=
+  | wf_prog_intro : forall
+      (Hwfcfg : wf_cfg g)
+      (Hwfis : forall p i, insn_at_pc g p i -> wf_insn g i p)
+      (Hwftmn : forall p' i, tmn_pc g p' -> insn_at_pc g p' i -> is_tmn i)
+      (Hwfentry : forall p, ~ succ_pc g p (block_entry (entry_block g))),
+      wf_prog g.
+
+End Typing.
+
+(** ** Correctness *)
+
+Module OpsemCorrect.
+  Import Typing Opsem.
+
+(** First, some utilities. *)
+(* HIDE *)
+(*
+  Lemma insn_at_pc_inj : forall g, wf_cfg g ->
+    injective (insn_at_pc g).
+(* FOLD *)
+  Proof.
+    intros g Hwfc. specialize (uid_at_pc_inj g Hwfc).
+    unfold injective, uid_at_pc. intros.
+    destruct b; eauto.
+  Qed.
+(* /FOLD *)
+*)
+(* /HIDE *)
+
+(* HIDE *)
+  (* LATER: Arguably the next two lemmas could go in the CFG module. *)
+(* /HIDE *)
+
+  Lemma uid_at_pc_func : forall g, wf_cfg g ->
+    functional (uid_at_pc g).
+(* FOLD *)
+  Proof.
+    intros g Hwfc. specialize (insn_at_pc_func g Hwfc).
+    unfold functional, uid_at_pc. intros.
+    destruct H0 as [c1 ?]. destruct H1 as [c2 ?].
+    cut ((b1,c1) = (b2,c2)). inversion 1; auto.
+    eauto.
+  Qed.
+(* /FOLD *)
+
+  Lemma eq_pc_uid : forall g pc id1 id2 c1 c2,
+    wf_prog g ->
+    insn_at_pc g pc (id1, c1) ->
+    insn_at_pc g pc (id2, c2) ->
+    id1 = id2.
+(* FOLD *)
+  Proof.
+    intros. inversion H. pose proof (uid_at_pc_func g Hwfcfg).
+    unfold functional in H2. eapply H2; red; eauto.
+  Qed.
+(* /FOLD *)
+
+(* HIDE *)
+  Unset Printing Records.
+(* /HIDE *)
+
+
+  (** *** Dominance relation *)
+
+  (** A more convenient form for typing rules *)
+
+  Lemma uid_sdom_step : forall g uid' uid pc1 pc2 c,
+    wf_prog g ->
+    uid' <> uid ->
+    wf_pc g pc2 ->
+    succ_pc g pc1 pc2 ->
+    insn_at_pc g pc1 (uid, c) ->
+    uid_sdom_pc g uid' pc2 ->
+    uid_sdom_pc g uid' pc1.
+(* FOLD *)
+  Proof.
+    unfold uid_sdom_pc. 
+    intros g uid' uid pc1 pc2 c Hwff Hneq Hpc Hsucc Hi [pc' [Hdef Hdom]]. 
+    exists pc'. split. assumption. 
+    split. contradict Hneq. subst pc'. 
+    destruct Hdef as [? [? ?]]; eapply eq_pc_uid; eauto. 
+    inversion Hwff; eapply dom_step; eauto. 
+  Qed.
+(* /FOLD *)
+
+  (** ** Progress & Preservation *)
+
+  (** Extend well-formedness definitions to include all components of 
+  the state. *)
+
+  Definition wf_loc (g:Cfg.t) (p:pc) (loc:loc) : Prop :=
+  forall uid, uid_sdom_pc g uid p -> exists n, loc uid = Some n.
+
+  Definition at_entry (g:Cfg.t) (p:pc) : Prop :=
+    entry_of_pc p = block_entry (entry_block g).
+
+  Inductive wf_state (g:Cfg.t) : state -> Prop :=
+  | wf_state_intro : forall st
+      (Hwfpc: wf_pc g st.(st_pc))
+      (Hwfloc: wf_loc g st.(st_pc) st.(st_loc))
+      (Hwfppc: at_entry g st.(st_pc) \/ 
+                 succ_pc g st.(st_ppc) (entry_of_pc st.(st_pc)))
+      (Hwfploc: at_entry g st.(st_pc) \/ 
+                  wf_loc g st.(st_ppc) st.(st_ploc)),
+      wf_state g st.
+
+  (** Initial state is well formed *)
+
+  Lemma wf_init_state : 
+    forall g m, wf_prog g ->
+    wf_state g (init_state g m).
+(* FOLD *)
+  Proof.
+    intros g m Hprog. inversion Hprog. 
+    apply wf_entry in Hwfcfg.
+    econstructor. auto.
+    red. simpl. intros. red in H. destruct H as [? [? [? ?]]].
+    red in H1. contradict H0.
+    cut (In x [block_entry (entry_block g)]). simpl. intuition.
+    eapply H1. econstructor. auto.
+    left. unfold init_state, at_entry, entry_of_pc. auto.
+    left. unfold init_state, at_entry, entry_of_pc. auto.
+  Qed.
+(* /FOLD *)  
+
+
+  (** *** Progress helper lemmas. *)
+
+  (** There are no phi nodes in the entry block. *)
+
+  Lemma at_entry_not_phi : forall g st i,
+    wf_prog g ->
+    at_entry g st.(st_pc) ->
+    insn_at_pc g st.(st_pc) i ->
+    ~ is_phi i.
+(* FOLD *)
+   Proof.
+     intros g st i Hprog Hentry Hinsn. 
+     destruct Hprog as [_ ? _ ?].
+     specialize (Hwfis _ _ Hinsn). inversion Hwfis; subst.
+     intro Hphi. specialize (H1 Hphi). destruct H1 as [? [? ?]].
+     destruct (insn_phis i) eqn:His. contradiction H3; auto.
+     assert (In p (insn_phis i)) as Hin. rewrite His. left; auto.
+     destruct p. apply H2 in Hin. destruct Hin as [pred [Hpred Ht0]].
+     specialize (Hwfentry pred). contradict Hwfentry. 
+     rewrite <- Hentry; auto.
+   Qed.
+(* /FOLD *)  
+
+  (** In a well-formed program with well-formed locals, evaluating
+  a value is never undefined. *)
+
+  Lemma eval_val__wf_loc : forall g pc loc i v,
+    wf_prog g ->
+    wf_loc g pc loc ->
+    insn_at_pc g pc i ->
+    In v (insn_uses i) ->
+    exists n, eval_val loc v = Some n.
+(* FOLD *)
+  Proof.
+    intros ? ? ? ? v Hwff Hwfloc Hi ?. 
+    destruct v as [uid | n].
+    simpl. inversion Hwff as [_ ? _]. apply Hwfis in Hi. 
+    destruct Hi as [? ? Huse]. specialize (Huse uid). 
+    lapply Huse; auto.
+    simpl; eauto.
+  Qed.
+(* /FOLD *)  
+
+  (** ** Progress *)
+
+  Definition FinalState (g:Cfg.t) (s:state) : Prop :=
+    exists uid, insn_at_pc g s.(st_pc) (uid, cmd_tmn tmn_ret).
+  
+  Lemma progress : forall g s,
+    wf_prog g -> wf_state g s ->
+    FinalState g s \/ exists s', step g s s'.
+(* FOLD *)
+  Proof.
+    intros g s Hwff Hwfs.
+    inversion Hwfs as [? Hwfpc]; subst. inversion Hwff.
+    pose proof (wf_pc_insn g Hwfcfg _ Hwfpc) as [[i c] Hi].
+    rename s into j. set (s:=j) in *. destruct j. 
+    destruct c.
+  
+    - (* Case "cmd_bop". *)
+    eelim (eval_val__wf_loc) with (v:=v) (loc:=st_loc0); eauto; simpl; auto.
+    eelim (eval_val__wf_loc) with (v:=v0) (loc:=st_loc0); eauto; simpl; auto.
+    intros n1 Heqn1 n2 Heqn2.
+    right. eexists. eapply step_bop; eauto. unfold eval_bop.
+    rewrite Heqn1, Heqn2. reflexivity. 
+
+    - (* Case "cmd_phi". *)
+    right. specialize (Hwfis _ _ Hi). inversion Hwfis; subst.
+    
+    destruct Hwfppc as [|Hwfppc]. 
+    exfalso; eapply at_entry_not_phi; eauto. simpl; trivial.
+    destruct Hwfploc as [|Hwfploc]. 
+    exfalso; eapply at_entry_not_phi; eauto. simpl; trivial.
+
+    destruct (H1 I) as [Hphi _]. clear H1.
+    specialize (Hphi st_ppc0 Hwfppc). destruct Hphi as [[v Hin] Hdom].
+
+    cut (exists v, assoc Lbl.eq_dec (lbl_of st_ppc0) l = Some v). intros [v' Hv].
+    cut (exists n, eval_val st_ploc0 v' = Some n). intros [n Hn].
+    eexists. eapply step_phi. eauto. unfold eval_phi.
+    rewrite Hv. rewrite Hn. reflexivity.
+  
+    destruct v' as [i' | n']. simpl in *. apply Hwfploc. apply Hdom. 
+    eapply assoc_in. apply Hv. simpl; eauto.
+    eapply in_assoc_some. apply Hin.
+  
+    - (* Case "cmd_tmn". *)
+    destruct t0.
+    * (*  SCase "tmn_jmp". *)
+      right. eexists. eapply step_tmn. eauto. reflexivity.
+
+    * (* SCase "tmn_cbr". *)
+      cut (exists n, eval_val st_loc0 v = Some n). intros [n Heqn].
+      right. eexists. eapply step_tmn. eauto. simpl. rewrite Heqn. reflexivity.
+      eapply eval_val__wf_loc; eauto. simpl; auto.
+
+    * (* SCase "tmn_ret". *)
+      left. red; eauto. 
+
+    - (* Case "cmd_load". *)
+    right. eexists. apply step_load; eauto.
+
+    - (* Case "cmd_store". *)
+    right. cut (exists n1, eval_val st_loc0 v = Some n1). 
+    intros [n1 Heqn1]. eexists. eapply step_store. eauto. eauto.
+    eapply eval_val__wf_loc; eauto. simpl; auto.
+  Qed.
+(* /FOLD *)
+
+  (** *** Some first steps towards preservation. *)
+
+  Lemma wf_pc_incr : forall g p i,
+    wf_prog g ->
+    wf_pc g p ->
+    insn_at_pc g p i ->
+    ~ is_tmn i ->
+    wf_pc g (incr_pc p).
+(* FOLD *)
+  Proof.
+    intros. inversion H. 
+    apply (wf_pc_tmn g Hwfcfg) in H0 as [pt [Ht Hle]].
+    eapply wf_pc_le_tmn; eauto.
+    inversion Hle; subst. destruct H0.
+    contradict H2. eapply Hwftmn; eauto. 
+    constructor; auto with arith.
+  Qed.
+(* /FOLD *)
+
+  Lemma eval_tmn_in_lbls : forall l loc t uid,
+    Some l = eval_tmn loc t -> In l (insn_lbls (uid, cmd_tmn t)).
+(* FOLD *)
+  Proof.
+    intros.
+    destruct t0; simpl in *.
+    inversion H; auto.
+    destruct (eval_val loc v). injection H. 
+      destruct n; eauto.
+      discriminate H. discriminate H.
+  Qed.
+(* /FOLD *)
+
+  (** *** More preservation helpers*)
+
+  Lemma not_def_sdom_step : forall g p1 p2 i uid,
+    wf_prog g ->
+    wf_pc g p2 ->
+    insn_at_pc g p1 i ->
+    ~ defs_uid i ->
+    succ_pc g p1 p2 ->
+    uid_sdom_pc g uid p2 ->
+    uid_sdom_pc g uid p1.
+(* FOLD *)
+  Proof. 
+    destruct i; intros. inversion H4 as [? [[? [? Ht]] ?]].
+    eapply uid_sdom_step; eauto. 
+    contradict Ht. subst t0. assert (x = p1). 
+    inversion H; eapply uid_at_pc_inj; try red; eauto. subst x.
+    replace (uid, x0) with (uid, c); trivial. 
+    inversion H; eapply insn_at_pc_func; eauto.
+  Qed.
+(* /FOLD *)    
+
+  Lemma wf_loc_succ : forall g p1 p2 loc uid n c,
+   wf_prog g ->
+   wf_pc g p2 ->
+   insn_at_pc g p1 (uid, c) ->
+   succ_pc g p1 p2 ->
+   wf_loc g p1 loc ->
+   wf_loc g p2 (update loc uid (Some n)).
+(* FOLD *)
+  Proof.
+    intros. red; intros. destruct (Uid.eq_dec uid0 uid). subst.
+    rewrite Locals.update_eq; eauto. reflexivity.
+    rewrite Locals.update_neq; eauto. apply H3.
+    eapply uid_sdom_step; eauto. 
+  Qed.
+(* /FOLD *)
+
+  (** ** Preservation *)
+
+  Lemma preservation : forall g s s',
+    wf_prog g ->
+    wf_state g s -> step g s s' -> wf_state g s'.
+(* FOLD *)
+  Proof.
+    intros g _ s' Hwff [s Hwfpc Hwfloc] Hstep.
+    inversion Hstep; subst; simpl in *.
+  
+    - (* Case "step_bop". *)
+    assert (wf_pc g (incr_pc pc0)) as Hwfpc' by (eapply wf_pc_incr; eauto).
+    constructor; simpl; try solve [destruct pc0; auto].
+    eapply wf_loc_succ; eauto. constructor.
+
+    - (* Case "step_phi". *)
+    assert (wf_pc g (incr_pc pc0)) as Hwfpc' by (eapply wf_pc_incr; eauto).
+    constructor; simpl; try solve [destruct pc0; auto].
+    eapply wf_loc_succ; eauto. constructor.
+  
+    - (* Case "step_tmn". *)
+    assert (wf_pc g (l', 0)) as Hwfpc'.
+      inversion Hwff as [_ Hwfi _]. specialize (Hwfi _ _ H).
+      inversion Hwfi. red in H2. apply H2. 
+      eauto. eapply eval_tmn_in_lbls. eauto.
+
+    assert (succ_pc g pc0 (l', 0)) as Hsucc.
+      econstructor. eauto. eapply eval_tmn_in_lbls. eauto.
+    constructor; simpl; eauto. red; intros. apply Hwfloc.
+    eapply not_def_sdom_step; eauto.
+
+    - (* Case "step_load". *)
+    assert (wf_pc g (incr_pc pc0)) as Hwfpc' by (eapply wf_pc_incr; eauto).
+    constructor; simpl; try solve [destruct pc0; auto].
+    eapply wf_loc_succ; eauto. constructor.
+
+    - (* Case "step_store". *)
+    assert (wf_pc g (incr_pc pc0)) as Hwfpc' by (eapply wf_pc_incr; eauto).
+    constructor; simpl; try solve [destruct pc0; auto].
+    red; intros. apply Hwfloc. eapply not_def_sdom_step; eauto. constructor.
+  Qed.
+(* /FOLD *)  
+
+(* HIDE *)
+Lemma step_deterministic : forall g s s1 s2, wf_prog g -> wf_state g s ->
+  step g s s1 -> step g s s2 -> s1 = s2.
+(* FOLD *)
+Proof.
+    intros g s s1 s2 Hwfprog Hwfs Hs1 Hs2.
+    inversion Hwfs as [? Hwfpc]; subst. inversion Hwfprog.
+    inversion Hs1; subst; simpl in *.
+
+    - (* Case "step_bop". *)
+    inversion Hs2; subst; simpl in *.
+    assert ((uid, cmd_bop bop0 v1 v2) = (uid0, cmd_bop bop1 v0 v3)).
+    apply (insn_at_pc_func g Hwfcfg pc0); auto. inversion H1; subst.
+    rewrite <- H8 in H0. inversion H0; subst. auto.
+
+    assert ((uid, cmd_bop bop0 v1 v2) = (uid0, cmd_phi pas)).
+    apply (insn_at_pc_func g Hwfcfg pc0); auto. inversion H1; subst.
+
+    assert ((uid, cmd_bop bop0 v1 v2) = (uid0, cmd_tmn tmn0)).
+    apply (insn_at_pc_func g Hwfcfg pc0); auto. inversion H1; subst.
+
+    assert ((uid, cmd_bop bop0 v1 v2) = (uid0, cmd_load addr)).
+    apply (insn_at_pc_func g Hwfcfg pc0); auto. inversion H1; subst.
+    
+    assert ((uid, cmd_bop bop0 v1 v2) = (uid0, cmd_store addr v)).
+    apply (insn_at_pc_func g Hwfcfg pc0); auto. inversion H1; subst.
+    
+    - (* Case "step_phi". *)
+    inversion Hs2; subst; simpl in *.
+
+    assert ((uid, cmd_phi pas) = (uid0, cmd_bop bop0 v1 v2)).
+    apply (insn_at_pc_func g Hwfcfg pc0); auto. inversion H1; subst.
+
+    assert ((uid, cmd_phi pas) = (uid0, cmd_phi pas0)).
+    apply (insn_at_pc_func g Hwfcfg pc0); auto. inversion H1; subst.
+    rewrite <- H8 in H0. inversion H0; subst; auto.
+
+    assert ((uid, cmd_phi pas) = (uid0, cmd_tmn tmn0)).
+    apply (insn_at_pc_func g Hwfcfg pc0); auto. inversion H1; subst.
+
+    assert ((uid, cmd_phi pas) = (uid0, cmd_load addr)).
+    apply (insn_at_pc_func g Hwfcfg pc0); auto. inversion H1; subst.
+    
+    assert ((uid, cmd_phi pas) = (uid0, cmd_store addr v)).
+    apply (insn_at_pc_func g Hwfcfg pc0); auto. inversion H1; subst.
+
+    - (* Case "step_tmn". *)
+    inversion Hs2; subst; simpl in *.
+
+    assert ((uid, cmd_tmn tmn0) = (uid0, cmd_bop bop0 v1 v2)).
+    apply (insn_at_pc_func g Hwfcfg pc0); auto. inversion H1; subst.
+
+    assert ((uid, cmd_tmn tmn0) = (uid0, cmd_phi pas)).
+    apply (insn_at_pc_func g Hwfcfg pc0); auto. inversion H1; subst.
+
+    assert ((uid, cmd_tmn tmn0) = (uid0, cmd_tmn tmn1)).
+    apply (insn_at_pc_func g Hwfcfg pc0); auto. inversion H1; subst.
+    rewrite <- H8 in H0. inversion H0; subst; auto.
+
+    assert ((uid, cmd_tmn tmn0) = (uid0, cmd_load addr)).
+    apply (insn_at_pc_func g Hwfcfg pc0); auto. inversion H1; subst.
+    
+    assert ((uid, cmd_tmn tmn0) = (uid0, cmd_store addr v)).
+    apply (insn_at_pc_func g Hwfcfg pc0); auto. inversion H1; subst.
+
+    - (* Case "step_load". *)
+    inversion Hs2; subst; simpl in *.
+
+    assert ((uid, cmd_load addr) = (uid0, cmd_bop bop0 v1 v2)).
+    apply (insn_at_pc_func g Hwfcfg pc0); auto. inversion H0; subst.
+
+    assert ((uid, cmd_load addr) = (uid0, cmd_phi pas)).
+    apply (insn_at_pc_func g Hwfcfg pc0); auto. inversion H0; subst.
+
+    assert ((uid, cmd_load addr) = (uid0, cmd_tmn tmn0)).
+    apply (insn_at_pc_func g Hwfcfg pc0); auto. inversion H0; subst.
+
+    assert ((uid, cmd_load addr) = (uid0, cmd_load addr0)).
+    apply (insn_at_pc_func g Hwfcfg pc0); auto. inversion H0; subst.
+    auto.
+
+    assert ((uid, cmd_load addr) = (uid0, cmd_store addr0 v)).
+    apply (insn_at_pc_func g Hwfcfg pc0); auto. inversion H0; subst.
+
+
+    - (* "step_store". *)
+    inversion Hs2; subst; simpl in *.
+
+    assert ((uid, cmd_store addr v) = (uid0, cmd_bop bop0 v1 v2)).
+    apply (insn_at_pc_func g Hwfcfg pc0); auto. inversion H1; subst.
+
+    assert ((uid, cmd_store addr v) = (uid0, cmd_phi pas)).
+    apply (insn_at_pc_func g Hwfcfg pc0); auto. inversion H1; subst.
+
+    assert ((uid, cmd_store addr v) = (uid0, cmd_tmn tmn0)).
+    apply (insn_at_pc_func g Hwfcfg pc0); auto. inversion H1; subst.
+
+    assert ((uid, cmd_store addr v) = (uid0, cmd_load addr0)).
+    apply (insn_at_pc_func g Hwfcfg pc0); auto. inversion H1; subst.
+
+    assert ((uid, cmd_store addr v) = (uid0, cmd_store addr0 v0)).
+    apply (insn_at_pc_func g Hwfcfg pc0); auto. inversion H1; subst.
+    rewrite <- H8 in H0. inversion H0. subst; auto.
+Qed.  
+(* /FOLD *)
+(* /HIDE *)
+
+End OpsemCorrect.
+
+Export Opsem Typing OpsemCorrect.
+
+End Make.
+
+(** *** List-based CFG Implementation *)
+
+(**  One possible implementation of cfgs *)
+
+Module ListCFG <: CFG.
+  Definition block := (lbl * list insn)%type.
+  Definition t := (lbl * list block)%type.
+  Local Notation cfg := t.
+
+  Definition entry_block : cfg -> lbl := @fst _ _.
+
+  Inductive wf_cfg' : cfg -> Prop :=
+    wf_cfg_intro : forall l bs,
+    NoDup (map (@fst _ _) bs) ->
+    NoDup (flat_map (fun b => map (@fst _ _) (snd b)) bs) ->
+    In l (map (@fst _ _) bs) ->
+    ~ In [] (map (@snd _ _) bs) ->
+    wf_cfg' (l, bs).
+
+  (* hack around some limitation re inductive types & parameters *)
+  Definition wf_cfg := wf_cfg'.
+
+  Lemma wf_cfg_block_len : forall g, wf_cfg g ->
+    forall l is, In (l, is) (snd g) -> length is <> 0.
+  Proof.
+    inversion 1. intros. destruct is; simpl; auto. 
+    contradict H2. 
+    eapply in_map with (f:=@snd _ _) in H5. auto.
+  Qed.
+
+  Definition wf_pc (g:cfg) (p:pc) : Prop :=
+    let (l, n) := p in
+    exists is i, In (l, is) (snd g) /\ Nth i is n.
+
+  Definition tmn_pc (g:cfg) (p:pc) : Prop :=
+    let (l, n) := p in
+    exists is, In (l, is) (snd g) /\ n = pred (length is).
+
+  Definition insn_at_pc (g:cfg) (p:pc) (i:insn) : Prop :=
+    let (l, n) := p in
+    exists is, In (l, is) (snd g) /\ Nth i is n.
+    
+  Definition uid_at_pc (g:cfg) (p:pc) (uid:uid) : Prop :=
+    exists c, insn_at_pc g p (uid, c).
+
+  Lemma wf_pc_insn : forall g, wf_cfg g ->
+    forall p, wf_pc g p -> exists i, insn_at_pc g p i.
+  Proof.
+    unfold wf_pc, insn_at_pc. destruct p; intros. 
+    decompose [ex and] H0. eauto.
+  Qed.
+
+  Lemma wf_pc_tmn : forall g, wf_cfg g ->
+    forall p, wf_pc g p -> exists p', tmn_pc g p' /\ le_pc p p'.
+  Proof.
+    unfold wf_pc, tmn_pc. destruct p. intros.
+    decompose [ex and] H0. 
+    exists (t0, pred (length x)). split. eauto.
+    constructor. 
+    apply PeanoNat.Nat.lt_le_pred.
+    eapply Nth_length; eauto.
+  Qed.
+
+  Lemma wf_pc_le_tmn : forall g, wf_cfg g ->
+    forall p', tmn_pc g p' -> forall p, le_pc p p' -> wf_pc g p.
+  Proof.
+    unfold wf_pc, tmn_pc. intros. destruct p, p'.
+    decompose [ex and] H0. exists x.
+
+    destruct x. apply wf_cfg_block_len in H3; auto. contradict H3; auto.
+    inversion H1; subst. apply le_lt_n_Sm in H5. 
+    erewrite <- S_pred in H5. 
+    apply length_Nth in H5 as [? ?]. 
+    eexists. split; eauto. eauto.
+  Qed.
+
+  Lemma wf_entry : forall g, wf_cfg g ->
+    wf_pc g (block_entry (entry_block g)).
+  Proof.
+    unfold wf_pc. inversion 1. simpl.
+    apply in_map_iff in H2 as [[? ?] [? ?]].
+    destruct l0.
+    exfalso. pose proof (wf_cfg_block_len g H t0 []) as contra. 
+    subst g; simpl in *. apply contra; auto.
+    eexists. eexists. 
+    simpl in *. subst l. split; eauto.
+    simpl; eauto.
+  Qed.
+
+  Lemma insn_at_pc_func : forall g, wf_cfg g ->
+    functional (insn_at_pc g).
+  Proof. 
+    unfold functional, insn_at_pc. inversion 1. destruct a.
+    intros b1 b2 [is1 [Hin1 Hnth1]] [is2 [Hin2 Hnth2]].
+    cut (is1 = is2). intro; subst is2. eapply Nth_eq; eauto.
+    eapply NoDup_assoc_func; eauto.
+  Qed.
+
+  Lemma uid_at_pc_inj : forall g, wf_cfg g ->
+    injective (uid_at_pc g).
+  Proof.
+    unfold injective, uid_at_pc, insn_at_pc. inversion 1.
+    intros [l1 n1] [l2 n2] uid [c1 [is1 [Hin1 Hnth1]]] [c2 [is2 [Hin2 Hnth2]]].
+    cut ((l1, is1) = (l2, is2)).
+    intro Heq. inversion Heq; clear Heq. f_equal.
+    eapply NoDup_flat_map__NoDup in H1; eauto.
+    change is1 with (snd (l1, is1)) in Hnth1.
+    change is2 with (snd (l2, is2)) in Hnth2.
+    subst; eapply NoDup_nth_inj; eauto. 
+
+    set (f1 b := map (@fst _ _) (snd b)) in *.
+    apply (NoDup_flat_map (l1, is1) (l2, is2) uid f1 bs); auto.
+    unfold f1; simpl. 
+    apply in_map_iff. exists (uid, c1); eauto using Nth_In.
+    apply in_map_iff. exists (uid, c2); eauto using Nth_In.
+  Qed.
+
+  (** ** Working with ListCFG. *)
+
+  (** Adds the given instruction list as a block labeled [l]. *)
+
+  Definition update (bs:list block) (l:lbl) (is:list insn) : list block :=
+    (l, is)::bs.
+
+  (** Lookup the block in the list. *)
+
+  Definition lookup (bs:list block) (l:lbl) : option (list insn) :=
+    assoc Lbl.eq_dec l bs.
+
+  (** ** Simple lemmas about CFG modifications. *)
+
+  Lemma update_eq :
+    forall (is : list insn) (l1 l2 : lbl) (bs : list block),
+      l1 = l2 -> lookup (update bs l1 is) l2 = Some is.
+  (* FOLD *)
+  Proof.
+    intros; unfold update, lookup.
+    subst. simpl. destruct (Lbl.eq_dec l2 l2); tauto.
+  Qed.
+  (* /FOLD *)
+
+  Lemma update_neq :
+    forall (l1 l2 : lbl) (is : list insn) (bs: list block),
+      l1 <> l2 -> lookup (update bs l1 is) l2 = lookup bs l2.
+  (* FOLD *)
+  Proof.
+    intros; subst; simpl.
+    destruct (Lbl.eq_dec l2 l1); subst; tauto.
+  Qed.
+  (* /FOLD *)
+
+
+End ListCFG.
+
